src/lowparse/LowParse.SteelSel.Access.fst
@@ -1,0 +1,106 @@
+module LowParse.SteelSel.Access
+include LowParse.SteelSel.VParse
+
+module S = Steel.Memory
+module SE = Steel.SelEffect
+module SEA = Steel.SelEffect.Atomic
+module A = Steel.SelArray
+module AP = Steel.SelArrayPtr
+
+module U32 = FStar.UInt32
+
+let parsed_size
+  (#k: parser_kind)
+  (#t: Type)
+  (p: parser k t)
+: Tot Type0
+= (a: byte_array) ->
+  SE.SteelSel U32.t
+    (vparse p a)
+    (fun _ -> vparse p a)
+    (fun _ -> True)
+    (fun h res h' ->
+      h' (vparse p a) == h (vparse p a) /\
+      U32.v res == A.length (h (vparse p a)).array
+    )
+
+let parsed_size_total_constant_size' // OK, but mostly not used
+  (#k: parser_kind)
+  (#t: Type)
+  (p: parser k t)
+  (sz: U32.t)
+: Pure (parsed_size p)
+    (requires (
+      k.parser_kind_subkind == Some ParserStrong /\
+      k.parser_kind_high == Some k.parser_kind_low /\
+      k.parser_kind_metadata == Some ParserKindMetadataTotal /\
+      U32.v sz == k.parser_kind_low
+    ))
+    (ensures (fun _ -> True))
+=
+  fun a ->
+  elim_vparse p a;
+  let _ = SEA.gget (AP.varrayptr a) in // FIXME: WHY WHY WHY is this needed?
+  parser_kind_prop_equiv k p;
+  intro_vparse p a;
+  SEA.return sz
+
+let strong_parsed_size
+  (#k: parser_kind)
+  (#t: Type)
+  (p: parser k t)
+: Tot Type0
+= (a: byte_array) ->
+  SE.SteelSel U32.t
+    (AP.varrayptr a)
+    (fun _ -> AP.varrayptr a)
+    (fun _ -> True)
+    (fun h res h' ->
+      let s = h (AP.varrayptr a) in
+      h' (AP.varrayptr a) == s /\
+      begin match parse p s.AP.contents with
+      | None -> False
+      | Some (_, consumed) -> U32.v res == consumed
+      end
+    )
+
+let get_parsed_size
+  (#k: parser_kind)
+  (#t: Type)
+  (#p: parser k t)
+  (j: strong_parsed_size p)
+: Tot (parsed_size p)
+=
+  fun a ->
+  elim_vparse p a;
+  let _ = SEA.gget (AP.varrayptr a) in // FIXME: WHY WHY WHY is this needed?
+  let res = j a in
+  intro_vparse p a;
+  SEA.return res
+
+let peek_strong
+  (#k: parser_kind)
+  (#t: Type)
+  (#p: parser k t)
+  (j: strong_parsed_size p)
+  (a: byte_array)
+: SE.SteelSel byte_array
+    (AP.varrayptr a)
+    (fun res -> vparse p a `SE.star` AP.varrayptr res)
+    (fun _ -> k.parser_kind_subkind == Some ParserStrong)
+    (fun h res h' ->
+      let c_a = h (AP.varrayptr a) in
+      let c_a' = h' (vparse p a) in
+      let c_res = h' (AP.varrayptr res) in
+      let consumed = A.length c_a'.array in
+      A.merge_into c_a'.array c_res.AP.array c_a.AP.array /\
+      is_byte_repr p c_a'.contents (Seq.slice c_a.AP.contents 0 consumed) /\
+      c_res.AP.contents == Seq.slice c_a.AP.contents consumed (A.length c_a.AP.array)
+    )
+=
+  let c_a = SEA.gget (AP.varrayptr a) in
+  let n = j a in
+  parse_strong_prefix p c_a.AP.contents (Seq.slice c_a.AP.contents 0 (U32.v n)); 
+  let res = AP.split a n in
+  intro_vparse p a;
+  SEA.return res
